Draft LPanic semantics

pancake/semantics/timeSemScript.sml
@@ -7,10 +7,15 @@ open preamble
 
 val _ = new_theory "timeSem";
 
+Datatype:
+  panic = PanicOutput
+        | PanicInput in_signal
+End
 
 Datatype:
   label = LDelay time
         | LAction ioAction
+        | LPanic panic
 End
 
 Datatype:
@@ -223,7 +228,8 @@ Inductive pickTerm:
     input_terms_actions max (Tm (Input in_signal) cnds clks dest diffs::tms) ∧
     terms_wtimes_ffi_bound m st (Tm (Input in_signal) cnds clks dest diffs::tms) ∧
     evalTerm st (SOME in_signal) (Tm (Input in_signal) cnds clks dest diffs) st' ⇒
-    pickTerm st max m (SOME in_signal) (Tm (Input in_signal) cnds clks dest diffs::tms) st') ∧
+    pickTerm st max m (SOME in_signal) (Tm (Input in_signal) cnds clks dest diffs::tms) st'
+             (LAction (Input in_signal))) ∧
 
   (!st max m cnds out_signal clks dest diffs tms st'.
     EVERY (λcnd. evalCond st cnd) cnds ∧
@@ -233,34 +239,43 @@ Inductive pickTerm:
     input_terms_actions max tms ∧
     terms_wtimes_ffi_bound m st (Tm (Output out_signal) cnds clks dest diffs::tms) ∧
     evalTerm st NONE (Tm (Output out_signal) cnds clks dest diffs) st' ⇒
-    pickTerm st max m NONE (Tm (Output out_signal) cnds clks dest diffs::tms) st') ∧
+    pickTerm st max m NONE (Tm (Output out_signal) cnds clks dest diffs::tms) st'
+             (LAction (Output out_signal))) ∧
 
-  (!st max m cnds event ioAction clks dest diffs tms st'.
+  (!st max m cnds event ioAction clks dest diffs tms st' lbl.
     EVERY (λcnd. EVERY (λe. ∃t. evalExpr st e = SOME t) (destCond cnd)) cnds ∧
     ~(EVERY (λcnd. evalCond st cnd) cnds) ∧
     tm_conds_eval_limit m st (Tm ioAction cnds clks dest diffs) ∧
     term_time_range m (Tm ioAction cnds clks dest diffs) ∧
     input_terms_actions max [(Tm ioAction cnds clks dest diffs)] ∧
     terms_wtimes_ffi_bound m st (Tm ioAction cnds clks dest diffs :: tms) ∧
-    pickTerm st max m event tms st' ⇒
-    pickTerm st max m event (Tm ioAction cnds clks dest diffs :: tms) st') ∧
+    pickTerm st max m event tms st' lbl ⇒
+    pickTerm st max m event (Tm ioAction cnds clks dest diffs :: tms) st' lbl) ∧
 
-  (!st max m cnds event in_signal clks dest diffs tms st'.
+  (!st max m cnds event in_signal clks dest diffs tms st' lbl.
     event <> SOME in_signal ∧
     tm_conds_eval_limit m st (Tm (Input in_signal) cnds clks dest diffs) ∧
     term_time_range m (Tm (Input in_signal) cnds clks dest diffs) ∧
     terms_wtimes_ffi_bound m st (Tm (Input in_signal) cnds clks dest diffs :: tms) ∧
     in_signal + 1 < max ∧
-    pickTerm st max m event tms st' ⇒
-    pickTerm st max m event (Tm (Input in_signal) cnds clks dest diffs :: tms) st') ∧
+    pickTerm st max m event tms st' lbl ⇒
+    pickTerm st max m event (Tm (Input in_signal) cnds clks dest diffs :: tms) st' lbl) ∧
 
-  (!st max m cnds event out_signal clks dest diffs tms st'.
+  (!st max m cnds event out_signal clks dest diffs tms st' lbl.
     event <> NONE ∧
     tm_conds_eval_limit m st (Tm (Output out_signal) cnds clks dest diffs) ∧
     term_time_range m (Tm (Output out_signal) cnds clks dest diffs) ∧
     terms_wtimes_ffi_bound m st (Tm (Output out_signal) cnds clks dest diffs :: tms) ∧
-    pickTerm st max m event tms st' ⇒
-    pickTerm st max m event (Tm (Output out_signal) cnds clks dest diffs :: tms) st')
+    pickTerm st max m event tms st' lbl ⇒
+    pickTerm st max m event (Tm (Output out_signal) cnds clks dest diffs :: tms) st' lbl) ∧
+
+  (!st max m.
+    max_clocks st.clocks m  ⇒
+    pickTerm st max m NONE [] st (LPanic PanicOutput)) ∧
+
+  (!st max m in_signal.
+    max_clocks st.clocks m  ⇒
+    pickTerm st max m (SOME in_signal) [] st (LPanic (PanicInput in_signal)))
 End
 
 (* m ≤ w + n *)
@@ -289,23 +304,61 @@ Inductive step:
           (SOME (w - d)))) ∧
 
   (!p m n st tms st' in_signal.
-      ALOOKUP p st.location = SOME tms ∧
-      n < m ∧
-      (case st.waitTime of
-       | NONE => T
-       | SOME wt => wt ≠ 0 ∧ wt < m) ∧
-      pickTerm (resetOutput st) m m (SOME in_signal) tms st' ∧
-      st'.ioAction = SOME (Input in_signal) ⇒
-      step p (LAction (Input in_signal)) m n st st') ∧
+    n < m ∧
+    ALOOKUP p st.location = SOME tms ∧
+    (case st.waitTime of
+     | NONE => T
+     | SOME wt => wt ≠ 0 ∧ wt < m) ∧
+    pickTerm (resetOutput st) m m (SOME in_signal) tms st' (LAction (Input in_signal)) ∧
+    st'.ioAction = SOME (Input in_signal) ⇒
+    step p (LAction (Input in_signal)) m n st st') ∧
 
   (!p m n st tms st' out_signal.
+    n < m ∧
     ALOOKUP p st.location = SOME tms ∧
     st.waitTime = SOME 0 ∧
-    n < m ∧
-    pickTerm (resetOutput st) m m NONE tms st' ∧
+    pickTerm (resetOutput st) m m NONE tms st' (LAction (Output out_signal)) ∧
     st'.ioAction = SOME (Output out_signal) ⇒
-    step p (LAction (Output out_signal)) m n st st')
+    step p (LAction (Output out_signal)) m n st st') ∧
+
+  (!p m n st tms st' in_signal.
+    n < m ∧
+    ALOOKUP p st.location = SOME tms ∧
+    (case st.waitTime of
+     | NONE => T
+     | SOME wt => wt ≠ 0 ∧ wt < m) ∧
+    pickTerm st m m (SOME in_signal) tms st' (LPanic (PanicInput in_signal)) ⇒
+    step p (LPanic (PanicInput in_signal)) m n st st') ∧
+
+  (!p m n st tms st'.
+    n < m ∧
+    ALOOKUP p st.location = SOME tms ∧
+    st.waitTime = SOME 0 ∧
+    pickTerm st m m NONE tms st' (LPanic PanicOutput) ⇒
+    step p (LPanic PanicOutput) m n st st')
 End
+
+(*
+  (!p m n st event tms st'.
+    n < m ∧
+    (case st.waitTime of
+     | NONE => T
+     | SOME wt => wt < m) ∧
+    ALOOKUP p st.location = SOME tms ∧
+    pickTerm st m m event tms st LPanic ⇒
+    step p LPanic m n st st')
+*)
+
+
+
+(*
+| StepPanic :
+    forall st act tms st',
+      lookup p (location st) = Some tms ->
+      pickTerm st act tms st' LPanic ->
+      step p LPanic st st'
+
+*)
 
 (*
 case s.waitTime of
@@ -357,5 +410,23 @@ Inductive stepTrace:
     stepTrace p m n st st'' (lbl::tr))
 End
 
+(*
+  (!st max m event tms p.
+    conds_eval_lt_dimword m st tms ∧
+    max_clocks st.clocks m ∧
+    terms_time_range m tms  ∧
+    input_terms_actions max tms ∧
+    terms_wtimes_ffi_bound m st tms ∧
+    EVERY (λtm.
+            EVERY
+            (λcnd. EVERY (λe. ∃t. evalExpr st e = SOME t) (destCond cnd))
+            (termConditions tm))
+          tms ∧
+    EVERY (λtm.
+            ~(EVERY (λcnd. evalCond st cnd) (termConditions tm)))
+          tms ⇒
+    pickTerm st max m event [] st (LPanic p))
+End
+*)
 
 val _ = export_theory();
